changed knows to derives and added the inital knowledge

SecurityNotation/Logic/logic.lean
@@ -7,11 +7,28 @@ import SecurityNotation.Basic.Syntax.Keys
 
 -- define the logic for the security notation
 -- need predicates: Knows, Honest, Fresh, Compromised, Trusted,
--- def knows (a : Principal) (m : Message) : Prop :=
 
+
+-- def knows (a : Principal) (m : Message) : Prop :=
 -- based on the Dolev-Yao Model
-inductive knows (initial_knowledge : Principal → Message → Prop) : Principal → Message → Prop where
-  | base : ∀ p m, initial_knowledge p m → knows initial_knowledge p m
-  | pair_unpack_l : ∀ p m1 m2, knows initial_knowledge p (Message.pair m1 m2) → knows initial_knowledge p m1
-  | pair_unpack_r : ∀ p m1 m2, knows initial_knowledge p (Message.pair m1 m2) → knows initial_knowledge p m2
-  | decrypt : ∀ p m k, knows initial_knowledge p (Message.enc m k) → knows initial_knowledge p (Message.key k) → knows initial_knowledge p m
+inductive derives (initial_knowledge : Principal → Message → Prop) : Principal → Message → Prop where
+  | base : ∀ p m, initial_knowledge p m → derives initial_knowledge p m
+  --analysis of the message
+  | pair_unpack_l : ∀ p m1 m2, derives initial_knowledge p (Message.pair m1 m2) → derives initial_knowledge p m1
+  | pair_unpack_r : ∀ p m1 m2, derives initial_knowledge p (Message.pair m1 m2) → derives initial_knowledge p m2
+  | decrypt : ∀ p m k, derives initial_knowledge p (Message.enc m k) → derives initial_knowledge p (Message.key k) → derives initial_knowledge p m
+  --creating a new message
+  | pair_pack : ∀ p m1 m2, derives initial_knowledge p m1 → derives initial_knowledge p m2 → derives initial_knowledge p (Message.pair m1 m2)
+  | encrypt : ∀ p m k, derives initial_knowledge p m → derives initial_knowledge p (Message.key k) → derives initial_knowledge p (Message.enc m k)
+
+
+-- this is the static knowledge that everyone knows before messaging
+inductive initial_knowledge (p : Principal) : Message → Prop where
+  -- this states that principal p knows all agents a
+  | knows_agents : ∀ (a : Principal), initial_knowledge p (Message.agent a)
+  -- this says that if the key is public they they can know it
+  | knows_public_keys : ∀ (k : Key), k.type = keyType.publicKey → initial_knowledge p (Message.key k)
+  -- this states that they will know their own private key
+  | knows_own_private_key : ∀ (k: Key), k.type = keyType.privateKey → k.owner = some p → initial_knowledge p (Message.key k)
+  -- this states that the principals know of everyone else who holds the key if they know it
+  | held_keys : ∀ (k : Key), p ∈ k.holders → initial_knowledge p (Message.key k)
